more vertical

theories/i2a_bij_vertical.v
@@ -14,6 +14,423 @@ Require Import refframe.imp_heap_bij_own.
 
 Local Open Scope Z_scope.
 
+Definition hb_priv_s' (bij : heap_bij) : gmap prov (gmap loc val) :=
+  ((λ '(HBIConstant x), x) <$> hb_priv_s bij).
+
+Definition val_through_bij (bij : heap_bij) (vs : val) : val :=
+  match vs with
+  | ValLoc l => ValLoc (if hb_bij bij !! l.1 is Some (HBShared p) then p else inhabitant, l.2)
+  | _ => vs
+  end.
+
+Program Definition heap_through_bij (bij : heap_bij) (h : heap_state) : heap_state :=
+  Heap (list_to_map $ omap (OMap:=list_omap) (λ '(l, v), if hb_bij bij !! l.1 is Some (HBShared p) then
+         Some ((p, l.2), val_through_bij bij v) else None) (map_to_list (h_heap h)))
+       (gset_to_gmap tt $ hb_shared_i bij) _.
+Next Obligation.
+  move => ??. apply bool_decide_spec. move => ? /elem_of_map[?[?/elem_of_dom]]. subst.
+  rewrite dom_gset_to_gmap.
+  rewrite list_to_map_lookup_is_Some => -[?]. rewrite elem_of_list_omap => -[[[??]?]]/=[??].
+  repeat case_match; simplify_eq. rewrite elem_of_hb_shared_i. naive_solver.
+Qed.
+
+Lemma heap_through_bij_provs bij h :
+  h_provs (heap_through_bij bij h) = hb_shared_i bij.
+Proof. by rewrite /h_provs dom_gset_to_gmap. Qed.
+
+Lemma heap_through_bij_Some bij h pi o vi:
+  h_heap (heap_through_bij bij h) !! (pi, o) = Some vi ↔
+    ∃ ps vs, hb_bij bij !! ps = Some (HBShared pi) ∧ h_heap h !! (ps, o) = Some vs ∧ vi = val_through_bij bij vs.
+Proof.
+  simpl. rewrite -elem_of_list_to_map. 2: {
+    rewrite list_fmap_omap. apply NoDup_omap_2_strong; [|apply NoDup_map_to_list].
+    move => [[??]?] [[??]?] [??] /=.
+    move => /elem_of_map_to_list ?/elem_of_map_to_list? /fmap_Some[[??][??]] /fmap_Some[[??][??]].
+    by repeat case_match; simplify_eq/=; simplify_bij.
+  }
+  rewrite elem_of_list_omap.
+  split.
+  - move => [[[??]?]]. rewrite elem_of_map_to_list => ?. repeat case_match => //; naive_solver.
+  - move => ?. destruct_all?. eexists (_,_,_). rewrite elem_of_map_to_list. split; [done|].
+    by simplify_option_eq.
+Qed.
+Opaque heap_through_bij.
+
+Lemma heap_through_bij_is_Some bij h pi o:
+  is_Some (h_heap (heap_through_bij bij h) !! (pi, o)) ↔
+          ∃ ps, hb_bij bij !! ps = Some (HBShared pi) ∧ is_Some (h_heap h !! (ps, o)).
+Proof. rewrite /is_Some. setoid_rewrite heap_through_bij_Some. naive_solver. Qed.
+
+Lemma heap_through_bij_is_Some' bij h pi ps o:
+  hb_bij bij !! ps = Some (HBShared pi) →
+  is_Some (h_heap (heap_through_bij bij h) !! (pi, o)) ↔ is_Some (h_heap h !! (ps, o)).
+Proof.
+  move => ?. rewrite heap_through_bij_is_Some. split; [|naive_solver].
+  move => [p'[??]]. by simplify_bij.
+Qed.
+
+Definition i2a_combine_bij (ih : gmap prov Z) (bij : heap_bij) : gmap prov Z :=
+  omap (λ v, if v is HBShared pi then
+               if ih !! pi is Some a then
+                 Some a
+               else
+                 None
+             else
+               None) bij.(hb_bij).
+
+Lemma i2a_combine_bij_lookup_Some ih bij p a:
+  i2a_combine_bij ih bij !! p = Some a ↔ ∃ p', hb_bij bij !! p = Some (HBShared p') ∧ ih !! p' = Some a.
+Proof.
+  rewrite /i2a_combine_bij lookup_omap_Some.
+  split => ?; destruct_all?.
+  - do 2 case_match => //. simplify_eq. naive_solver.
+  - eexists (HBShared _). by simplify_map_eq.
+Qed.
+
+Lemma i2a_combine_extend iha bijb ih ho h :
+  i2a_combine_bij (i2a_ih_shared iha) bijb ⊆ i2a_ih_shared ih →
+  ho ⊆ hb_priv_s' bijb →
+  ho ⊆ i2a_ih_constant ih →
+  i2a_heap_agree h ih →
+  ∃ ih' bijb',
+    i2a_ih_shared ih = i2a_combine_bij (ih' ∪ i2a_ih_shared iha) bijb' ∧
+    (I2AShared <$> ih') ##ₘ iha ∧
+    ho ⊆ hb_priv_s' bijb' ∧
+    heap_preserved (hb_priv_s bijb') h ∧
+    hb_shared bijb ⊆ hb_shared bijb' ∧
+    hb_priv_i bijb = hb_priv_i bijb'
+.
+Proof.
+Admitted.
+
+Lemma i2a_heap_shared_lookup_big1 m h :
+  i2a_heap_auth h -∗
+  ([∗ map] p↦a∈m, i2a_heap_shared p a) -∗
+  ⌜m ⊆ i2a_ih_shared h⌝.
+Proof.
+  iIntros "Ha Hm".
+  iInduction m as [|a v m' ?] "IH" using map_ind. { iPureIntro. apply map_empty_subseteq. }
+  rewrite big_sepM_insert //. iDestruct "Hm" as "[Hv Hm]".
+  iDestruct (i2a_heap_shared_lookup' with "[$] [$]") as %?.
+  iDestruct ("IH" with "[$] [$]") as %?. iPureIntro.
+  apply insert_subseteq_l; [|done]. by apply i2a_ih_shared_Some.
+Qed.
+
+Lemma i2a_heap_lookup_big1 m h :
+  i2a_heap_auth h -∗
+  ([∗ map] p↦b∈m, i2a_heap_constant p b) -∗
+  ⌜m ⊆ i2a_ih_constant h⌝.
+Proof.
+  iIntros "Ha Hm".
+  iInduction m as [|a v m' ?] "IH" using map_ind. { iPureIntro. apply map_empty_subseteq. }
+  rewrite big_sepM_insert //. iDestruct "Hm" as "[Hv Hm]".
+  iDestruct (i2a_heap_lookup' with "[$] [$]") as %?.
+  iDestruct ("IH" with "[$] [$]") as %?. iPureIntro.
+  apply insert_subseteq_l; [|done]. by apply i2a_ih_constant_Some.
+Qed.
+
+Lemma i2a_mem_update_all2 moa mem mo :
+  mo ⊆ mem →
+  moa ##ₘ mo →
+  i2a_mem_auth (moa ∪ mo) -∗
+  i2a_mem_map moa ==∗
+  i2a_mem_auth mem ∗ i2a_mem_map (mem ∖ mo).
+Proof.
+  iIntros (Hsub Hdisj) "Hmem Hconst".
+  iInduction moa as [|a v moa ?] "IH" using map_ind forall (mem mo Hsub Hdisj). {
+    rewrite left_id_L.
+    iMod (i2a_mem_alloc_big' with "[$]") as "[? $]". { apply map_disjoint_difference_l'. }
+    rewrite map_union_comm. 2: { apply map_disjoint_difference_l'. }
+    by rewrite map_difference_union.
+  }
+  move: Hdisj => /map_disjoint_insert_l [??].
+  rewrite {3}/i2a_mem_map big_sepM_insert //. iDestruct "Hconst" as "[Hc Hconst]".
+  rewrite -insert_union_l insert_union_r //.
+  iMod ("IH" $! (<[a:=v]> mem) with "[%] [%] [$] [$]") as "[Hmem Hconst]".
+  { by apply insert_mono. } { by apply map_disjoint_insert_r. }
+  rewrite (difference_insert _ _ _ _ _ v) -delete_difference.
+  destruct (mem !! a) as [v'|] eqn:?.
+  - iMod (i2a_mem_update' v' with "[$]") as "[??]". iModIntro.
+    rewrite insert_insert (insert_id _ _ v') //. iFrame.
+    iApply big_sepM_delete; [|by iFrame]. by apply lookup_difference_Some.
+  - rewrite delete_notin. 2: { apply lookup_difference_None. by left. } iFrame.
+    iMod (i2a_mem_delete' with "[$]"). by rewrite delete_insert.
+Qed.
+
+Lemma i2a_mem_update_all1 mem mem' mo :
+  mo ⊆ mem →
+  mo ⊆ mem' →
+  i2a_mem_auth mem' -∗
+  i2a_mem_map (mem' ∖ mo) ==∗
+  i2a_mem_auth mem ∗ i2a_mem_map (mem ∖ mo).
+Proof.
+  iIntros (Hsub ?) "Hmem Hconst".
+  iApply (i2a_mem_update_all2 (mem' ∖ mo) with "[Hmem] [$]").
+  { done. } { apply map_disjoint_difference_l'. }
+  rewrite map_union_comm. 2: { apply map_disjoint_difference_l'. }
+  by rewrite map_difference_union.
+Qed.
+
+Lemma i2a_heap_alloc_shared1 ih p a:
+  ih !! p = None →
+  i2a_heap_auth ih ==∗ i2a_heap_auth (<[p := I2AShared a]> ih) ∗ i2a_heap_shared p a.
+Proof.
+  iIntros (?) "?".
+  iMod (i2a_heap_alloc' _ _ ∅ with "[$]"); [done|].
+  iMod (i2a_heap_to_shared' with "[$]"). iModIntro. by rewrite insert_insert.
+Qed.
+
+Lemma i2a_heap_alloc_shared_big1 ih ih' :
+  (I2AShared <$> ih') ##ₘ ih →
+  i2a_heap_auth ih ==∗ i2a_heap_auth ((I2AShared <$> ih') ∪ ih) ∗ [∗ map] p↦a∈ih', i2a_heap_shared p a.
+Proof.
+  iIntros (?) "Hh".
+  iInduction ih' as [|p a ih' ?] "IH" using map_ind;
+    rewrite ->?fmap_empty, ?fmap_insert in *; decompose_map_disjoint.
+  { rewrite left_id big_sepM_empty. by iFrame. }
+  iMod ("IH" with "[//] [$]") as "[??]". rewrite -insert_union_l.
+  iMod (i2a_heap_alloc_shared1 with "[$]") as "[$ ?]".
+  { apply lookup_union_None. split!. rewrite lookup_fmap. by apply fmap_None. }
+  rewrite big_sepM_insert //. by iFrame.
+Qed.
+
+Definition i2a_val_rel_pure (ih : gmap prov prov) (iv : val) (av : Z) : Prop :=
+  match iv with
+  | ValNum z => av = z
+  | ValBool b => av = bool_to_Z b
+  | ValLoc l => ∃ z, av = (z + l.2)%Z ∧ ih !! l.1 = Some z
+  end.
+
+Lemma i2a_val_rel_to_pure v av ih :
+  i2a_heap_auth ih -∗
+  i2a_val_rel v av -∗
+  ⌜i2a_val_rel_pure (i2a_ih_shared ih) v av⌝.
+Proof.
+  iIntros "Hh Hv". destruct v => //=. iDestruct!.
+  iDestruct (i2a_heap_shared_lookup' with "[$] [$]") as %?.
+  iPureIntro. setoid_rewrite i2a_ih_shared_Some. naive_solver.
+Qed.
+
+Lemma i2a_val_rel_of_pure ih v av :
+  i2a_val_rel_pure ih v av →
+  ([∗ map] p↦a ∈ ih, i2a_heap_shared p a) -∗
+  i2a_val_rel v av.
+Proof.
+  iIntros (Hv) "Hsh". destruct v => //=. simplify_eq/=. destruct_all?. simplify_eq.
+  iSplit!; [done|]. by iApply (big_sepM_lookup with "[$]").
+Qed.
+
+Lemma i2a_val_rel_pure_through_bij iv av ih1 ih2 bij:
+  i2a_val_rel_pure ih1 iv av →
+  ih1 = i2a_combine_bij ih2 bij →
+  i2a_val_rel_pure ih2 (val_through_bij bij iv) av.
+Proof.
+  move => Hp ?. subst. destruct iv => //; simplify_eq/=.
+  move: Hp => [? [? /i2a_combine_bij_lookup_Some[?[??]]]]. simplify_map_eq.
+  naive_solver.
+Qed.
+
+Definition i2a_args_pure (ih : gmap prov prov) (o : nat) (vs : list val) (rs : gmap string Z) : Prop :=
+  ∀ i v, vs !! i = Some v → ∃ r av,
+      args_registers !! (o + i)%nat = Some r ∧
+      rs !! r = Some av ∧
+      i2a_val_rel_pure ih v av.
+
+Lemma i2a_args_to_pure ih o vs rs :
+  i2a_heap_auth ih -∗
+  i2a_args o vs rs -∗
+  ⌜i2a_args_pure (i2a_ih_shared ih) o vs rs⌝.
+Proof.
+  iIntros "Hh Hargs".
+  iInduction vs as [|v vs] "IH" forall (o). { iPureIntro => ? [] //. }
+  rewrite /i2a_args /=. iDestruct "Hargs" as "[[% [% [% [% ?]]]]?]".
+  iDestruct (i2a_val_rel_to_pure with "[$] [$]") as %?.
+  setoid_rewrite <-Nat.add_succ_comm.
+  iDestruct ("IH" with "[$] [$]") as %Hp.
+  iPureIntro => i ? /lookup_cons_Some[[??]|[? Hv]]; simplify_eq. 1: naive_solver. destruct i; [lia|].
+  setoid_rewrite <-Nat.add_succ_comm. apply Hp. rewrite -Hv. f_equal. lia.
+Qed.
+
+Lemma i2a_args_of_pure ih o vs rs :
+  i2a_args_pure ih o vs rs →
+  ([∗ map] p↦a ∈ ih, i2a_heap_shared p a) -∗
+  i2a_args o vs rs.
+Proof.
+  iIntros (Hp) "Hsh".
+  iInduction vs as [|v vs] "IH" forall (o Hp). { by rewrite /i2a_args /=. }
+  rewrite /i2a_args /=. iSplit.
+  - move: (Hp 0%nat v) => []// ?[?[?[??]]]. iSplit!. by iApply i2a_val_rel_of_pure.
+  - setoid_rewrite <-Nat.add_succ_comm. iApply ("IH" with "[%] [$]").
+    move => ???. setoid_rewrite Nat.add_succ_comm. by apply: Hp.
+Qed.
+
+Lemma i2a_args_pure_through_bij o vs rs ih1 ih2 bij:
+  i2a_args_pure ih1 o vs rs →
+  ih1 = i2a_combine_bij ih2 bij →
+  i2a_args_pure ih2 o (val_through_bij bij <$> vs) rs.
+Proof.
+  move => Hp ?. subst.
+  elim: vs o Hp; csimpl. { move => ?? ? []//. }
+  move => v ? IH ? Hp i v' /lookup_cons_Some[[??]|[? Hv]]; simplify_eq.
+  - move: (Hp 0%nat v) => []// ?[?[?[??]]]. split!. by apply: i2a_val_rel_pure_through_bij.
+  - destruct i; [lia|]. setoid_rewrite <-Nat.add_succ_comm. apply IH.
+    + move => ???. setoid_rewrite Nat.add_succ_comm. by apply Hp.
+    + rewrite -Hv. f_equal. lia.
+Qed.
+
+Definition i2a_heap_shared_agree_pure (h : gmap loc val) (ih : gmap prov prov) (mem : gmap Z (option Z)) : Prop :=
+  ∃ m2l : gmap Z loc,
+  map_Forall (λ l v,
+               if ih !! l.1 is Some a then
+                 ∃ av, i2a_val_rel_pure ih v av ∧ mem !! (a + l.2) = Some (Some av) ∧ m2l !! (a + l.2) = Some l
+               else True
+  ) h.
+
+
+Lemma i2a_heap_shared_agree_to_pure h ih :
+  i2a_heap_shared_agree h ih -∗
+  i2a_heap_auth ih -∗
+  ∃ m, ⌜i2a_heap_shared_agree_pure h (i2a_ih_shared ih) m⌝ ∗ i2a_mem_map m ∗ i2a_heap_auth ih.
+Proof.
+Admitted.
+
+Lemma i2a_heap_shared_agree_of_pure ih h m :
+  i2a_heap_shared_agree_pure h (i2a_ih_shared ih) m →
+  ([∗ map] p↦a ∈ i2a_ih_shared ih, i2a_heap_shared p a) -∗
+  i2a_mem_map m -∗
+  i2a_heap_shared_agree h ih.
+Proof.
+Admitted.
+
+
+
+(* Lemma i2a_heap_update_all1 bij bij': *)
+(*   i2a_bij_shared bij ⊆ i2a_bij_shared bij' → *)
+(*   i2a_bij_constant bij = i2a_bij_constant bij' → *)
+(*   i2a_heap_auth bij -∗ *)
+(*   ([∗ map] p↦a ∈ i2a_bij_shared bij, i2a_heap_shared p a) ==∗ *)
+(*   i2a_heap_auth bij' ∗ ([∗ map] p↦a ∈ i2a_bij_shared bij', i2a_heap_shared p a). *)
+(* Proof. *)
+(*   iIntros (??) "Ha Hbij". *)
+
+(* Lemma i2a_guard_page_decompose gp : *)
+  (* i2a_guard_page gp ⊣⊢ [∗ map] a↦v *)
+
+Lemma i2a_mem_transfer mem m1 m2 P1 P2:
+  satisfiable (i2a_mem_auth mem ∗ i2a_mem_map m1 ∗ i2a_mem_map m2 ∗ P1) →
+  satisfiable (i2a_mem_map (mem ∖ m1) ∗ P2) →
+    satisfiable (i2a_mem_auth mem ∗ i2a_mem_map (m2 ∪ m1) ∗ P1) ∧
+    satisfiable (i2a_mem_map m2 ∗ i2a_mem_map (mem ∖ (m2 ∪ m1)) ∗ P2).
+Proof.
+  move => Hs1 Hs2.
+  iSatStart Hs1. iIntros "(Hauth&Hm1&Hm2&?)".
+  iDestruct (i2a_mem_lookup_big' with "Hauth Hm1") as %?.
+  iDestruct (i2a_mem_lookup_big' with "Hauth Hm2") as %?.
+  iDestruct (i2a_mem_map_excl with "Hm1 Hm2") as %?.
+  iSatStop Hs1. split.
+  - iSatMono Hs1. iFrame. rewrite /i2a_mem_map big_sepM_union; [by iFrame|done].
+  - iSatMono Hs2. iIntros "(Hmem&$)".
+    rewrite -(map_difference_union m2 (mem ∖ m1)). 2: {
+      apply map_subseteq_spec => ???. apply lookup_difference_Some.
+      split; [by apply: lookup_weaken| by apply: map_disjoint_Some_l].
+    }
+    rewrite /i2a_mem_map big_sepM_union; [|by apply map_disjoint_difference_r'].
+    by rewrite map_difference_difference map_union_comm.
+Qed.
+
+
+Lemma heap_bij_update_all bij bij' ho :
+  ho ⊆ hb_priv_s' bij' →
+  ho ⊆ hb_priv_s' bij →
+  hb_shared bij' ⊆ hb_shared bij →
+  hb_priv_i bij' = hb_priv_i bij →
+  heap_bij_auth bij' -∗
+  ([∗ map] p2↦p1∈ hb_shared bij', heap_bij_shared p1 p2) -∗
+  ([∗ map] p↦h∈ hb_priv_s' bij' ∖ ho, heap_bij_const_s p h) ==∗
+  heap_bij_auth bij ∗
+  ([∗ map] p2↦p1∈ hb_shared bij, heap_bij_shared p1 p2) ∗
+  ([∗ map] p↦h∈ hb_priv_s' bij ∖ ho, heap_bij_const_s p h).
+Proof.
+  iIntros (????) "Hauth Hsh Hho".
+Admitted.
+(*   iApply (i2a_mem_update_all2 (mem' ∖ mo) with "[Hmem] [$]"). *)
+(*   { done. } { apply map_disjoint_difference_l'. } *)
+(*   rewrite map_union_comm. 2: { apply map_disjoint_difference_l'. } *)
+(*   by rewrite map_difference_union. *)
+(* Qed. *)
+
+Definition val_in_bij_pure (bij : heap_bij) (v1 v2 : val) : Prop :=
+  match v1, v2 with
+  | ValNum n1, ValNum n2 => n1 = n2
+  | ValBool b1, ValBool b2 => b1 = b2
+  | ValLoc l1, ValLoc l2 => l1.2 = l2.2 ∧ hb_bij bij !! l2.1 = Some (HBShared l1.1)
+  | _, _ => False
+  end.
+
+Lemma val_in_bij_to_pure bij v1 v2 :
+  heap_bij_auth bij -∗
+  val_in_bij v1 v2 -∗
+  ⌜val_in_bij_pure bij v1 v2⌝.
+Proof.
+  iIntros "Hh Hv". destruct v1, v2 => //=. unfold loc_in_bij. iDestruct!.
+  iDestruct (heap_bij_shared_lookup with "[$] [$]") as %?. done.
+Qed.
+
+Lemma val_in_bij_of_pure bij v1 v2 :
+  val_in_bij_pure bij v1 v2 →
+  ([∗ map]p2↦p1∈hb_shared bij, heap_bij_shared p1 p2) -∗
+  val_in_bij v1 v2.
+Proof.
+  iIntros (Hv) "Hsh". destruct v1, v2 => //=. simplify_eq/=. destruct_all?.
+  iSplit; [done|]. iApply (big_sepM_lookup with "[$]"). by apply hb_shared_lookup_Some.
+Qed.
+
+Definition heap_in_bij_pure (bij : heap_bij) (h h' : heap_state) : Prop :=
+  ∀ p1 p2 o,
+  hb_bij bij !! p2 = Some (HBShared p1) →
+
+  (is_Some (h.(h_heap) !! (p1, o)) ↔ is_Some (h'.(h_heap) !! (p2, o)))
+  ∧
+  ∀ v1 v2,
+  h.(h_heap)  !! (p1, o) = Some v1 →
+  h'.(h_heap) !! (p2, o) = Some v2 →
+  val_in_bij_pure bij v1 v2.
+
+Lemma heap_in_bij_to_pure bij h h' :
+  heap_bij_auth bij -∗
+  heap_in_bij bij h h' -∗
+  ⌜heap_in_bij_pure bij h h'⌝.
+Proof.
+  iIntros "Ha Hh". iIntros (????).
+  iDestruct ("Hh" with "[//]") as (?) "Hh".
+  iSplit; [done|]. iIntros (????).
+  iApply (val_in_bij_to_pure with "[$]"). by iApply "Hh".
+Qed.
+
+Lemma heap_in_bij_of_pure bij h h' :
+  heap_in_bij_pure bij h h' →
+  ([∗ map]p2↦p1∈hb_shared bij, heap_bij_shared p1 p2) -∗
+  heap_in_bij bij h h'.
+Proof.
+  iIntros (Hh) "Hsh". iIntros (p1 p2 o ?).
+  move: Hh => /(_ _ _ o ltac:(done))[? {}Hh]. iSplit; [done|].
+  iIntros (????). iApply (val_in_bij_of_pure with "[$]"). by apply: Hh.
+Qed.
+
+Lemma val_in_through_bij bij v av ih1 ih:
+  i2a_val_rel_pure ih1 v av →
+  ih1 = i2a_combine_bij ih bij →
+  ([∗ map] p2↦p1 ∈ hb_shared bij, heap_bij_shared p1 p2) -∗
+  val_in_bij (val_through_bij bij v) v.
+Proof.
+  iIntros (Hp ?) "Hbij". destruct v => //; simplify_eq/=.
+  move: Hp => [?[? /i2a_combine_bij_lookup_Some [?[??]]]]. simplify_map_eq.
+  iSplit; [done|]. iApply (big_sepM_lookup with "[$]").
+  by apply hb_shared_lookup_Some.
+Qed.
+
+
+
 Lemma i2a_bij_vertical m σ `{!VisNoAll m} ins fns f2i gp:
   trefines (MS (imp_to_asm ins fns f2i gp (imp_heap_bij m))
                (initial_imp_to_asm_state (imp_heap_bij m) (initial_imp_heap_bij_state m σ)))
@@ -25,26 +442,212 @@ Proof.
     exact (λ pl '(I2A csa lra) _ '(I2A cs lr) Pa Pb P,
       csa = cs ∧
       lra = lr ∧
+      ∃ mem' moa mo,
+        (* mem' = moa ∪ mo ∧ *)
     if pl is Env then
-      True
+      ∃ iha bijb hob ho hprev,
+        moa = mem' ∖ mo ∧
+        mo ⊆ mem' ∧
+        hob = hb_priv_s' bijb ∖ ho ∧
+        ho ⊆ hb_priv_s' bijb ∧
+        i2a_heap_agree hprev iha ∧
+        heap_preserved (hb_priv_i bijb) hprev ∧
+        (P ⊣⊢ ([∗ map] a↦v ∈ mo, i2a_mem_constant a v) ∗
+           ([∗ map] p↦a ∈ i2a_combine_bij (i2a_ih_shared iha) bijb, i2a_heap_shared p a) ∗
+           ([∗ map] p↦h ∈ ho, i2a_heap_constant p h)) ∧
+        satisfiable (Pa ∗
+                        i2a_mem_auth mem' ∗ i2a_heap_auth iha ∗
+                        i2a_mem_map moa ∗
+                        ([∗ map]p↦a ∈ i2a_ih_shared iha, i2a_heap_shared p a)) ∧
+        satisfiable (Pb ∗ heap_bij_auth bijb ∗
+           ([∗ map] p2↦p1∈ hb_shared bijb, heap_bij_shared p1 p2) ∗
+           ([∗ map] p↦h∈ hob, heap_bij_const_s p h))
     else
-      True
+      ∃ ih',
+        mo = mem' ∖ moa ∧
+        satisfiable (P ∗ i2a_mem_auth mem' ∗ i2a_heap_auth ih' ∗ i2a_mem_map mo ∗
+                        ([∗ map] p↦a ∈ i2a_ih_shared ih', i2a_heap_shared p a)) ∧
+        moa ⊆ mem' ∧
+        (Pa ⊣⊢ i2a_mem_map moa) ∧
+        (Pb ⊣⊢ True)
 ). }
-  { split!. }
+  { split!. all: admit. }
   all: move => [csa lra] [] [cs lr] Pa Pb P [? e] ?/=; destruct_all?; simplify_eq.
   - move: e => []//= pc regs mem b ? h. move: b => [] /=.
-    + move => i f args ???? P' HP'. eexists true => /=.
-      (* split!. *)
-      admit.
-    + move => v av rs' cs' ?? P' HP'. eexists false => /=. simplify_eq.
-      (* split!. *)
-      admit.
-  - move => vs hb' Pb' HPb' ? i rs' mem'.
+    + move => i f args ???? P' HP'. eexists true => /=. setoid_subst.
+      rename select (satisfiable (Pa ∗ _)) into HPa.
+      rename select (satisfiable (Pb ∗ _)) into HPb.
+      rename select (i2a_heap_agree hprev iha) into Hpreva.
+      rename select (heap_preserved (hb_priv_i bijb) hprev) into Hprevb.
+      iSatStart HP'. iIntros!.
+      iDestruct select (i2a_mem_inv _ _ _) as (?) "(Hgp&Hsp&Hmauth)".
+      iDestruct (i2a_mem_lookup_big' mo with "[$] [$]") as %?.
+      iDestruct (i2a_mem_uninit_alt1 with "[$]") as (? Hvslen) "Hsp"; [lia|].
+      iDestruct select (i2a_heap_inv _) as (ih ?) "[Hsh [Hhag Hh]]".
+      iDestruct (i2a_heap_shared_lookup_big1 (i2a_combine_bij _ _) with "[$] [$]") as %?.
+      iDestruct (i2a_heap_lookup_big1 with "[$] [$]") as %?.
+      iDestruct (i2a_heap_shared_agree_to_pure with "[$] [$]") as (??) "[? ?]".
+      iDestruct (i2a_args_to_pure with "[$] [$]") as %?.
+      iSatStop HP'.
+
+      have [//|//|//|//|ih' [bijb' ?]]:= i2a_combine_extend iha bijb ih ho h. destruct_all?.
+
+      iSatStartBupd HPa. iIntros!.
+      iMod (i2a_mem_update_all1 mem with "[$] [$]") as "[Ha Hmo]"; [done..|].
+      iMod (i2a_heap_alloc_shared_big1 with "[$]") as "[Hih ?]"; [done..|]. iModIntro.
+      iSatStop HPa.
+      efeed pose proof i2a_mem_transfer as H'.
+      2: { iSatMono HPa. iFrame. iAccu. }
+      { iSatMono HP'. iFrame. iAccu. }
+      clear HPa HP'. move: H' => [HP' HPa].
+      efeed pose proof i2a_mem_transfer as H'.
+      2: { iSatMono HPa. iIntros!. iFrame. iAccu. }
+      { iSatMono HP'. iIntros!. iFrame. iAccu. }
+      clear HPa HP'. move: H' => [HP' HPa].
+      efeed pose proof i2a_mem_transfer as H'.
+      2: { iSatMono HPa. iIntros!. iFrame. iAccu. }
+      { iSatMono HP'. iIntros!. iFrame. iAccu. }
+      clear HPa HP'. move: H' => [HP' HPa].
+
+      iSatStartBupd HPb. iIntros!.
+      iMod (heap_bij_update_all bijb' with "[$] [$] [$]") as "(Ha&Hsh&Hho)"; [done..|]. iModIntro.
+      iSatStop HPb.
+
+      split; [done|].
+      eexists (heap_merge (heap_restrict (heap_through_bij bijb' h)
+                                         (λ p, p ∈ dom (gset _) (ih' ∪ i2a_ih_shared iha)))
+                  (heap_restrict hprev
+                                 (λ x, x ∉ dom (gset _) (ih' ∪ i2a_ih_shared iha) ∨ x ∉ hb_shared_i bijb'))).
+      eexists _, _, (val_through_bij bijb' <$> args).
+      split!.
+      * iSatMono HPa. iIntros!.
+        iDestruct select (i2a_mem_map (mem ∖ _)) as "$". iFrame.
+        rewrite -!(assoc bi_sep). iSplit; [done|].
+        iDestruct (i2a_mem_uninit_alt2 with "[$]") as "Huninit". rewrite Hvslen Z2Nat.id; [|lia].
+        iFrame "Huninit".
+        rewrite !bi.sep_exist_r. iExists _.
+        rewrite -!(assoc bi_sep).
+        iDestruct select (i2a_heap_auth _) as "$".
+        iAssert ([∗ map] p↦a ∈ i2a_ih_shared ((I2AShared <$> ih') ∪ iha), i2a_heap_shared p a)%I as "#$". {
+          admit.
+        }
+
+        iSplit!.
+        -- split.
+           ++ rewrite heap_merge_provs !heap_restrict_provs dom_union_L. admit.
+           ++ move => /= ?? /lookup_union_Some_raw. rewrite lookup_fmap.
+              move => [/fmap_Some[?[?//]]|[/fmap_None ??]]. rewrite lookup_union_r. 2: {
+                apply map_filter_lookup_None. right => ?? /=. admit. }
+              rewrite map_filter_lookup_true; [by apply Hpreva|].
+              admit.
+        -- admit. (* TODO, not clear yet *)
+        -- iApply (i2a_args_of_pure (ih' ∪ i2a_ih_shared iha)).
+           ++ by apply: i2a_args_pure_through_bij.
+           ++ by iApply (big_sepM_union_2 with "[$]").
+      * iSatMono HPb. iIntros!. iFrame. iSplit!.
+        -- iExists _. iFrame. repeat iSplit.
+           ++ iPureIntro. admit.
+           ++ iPureIntro. rewrite heap_merge_provs !heap_restrict_provs. admit.
+           ++ done.
+           ++ iPureIntro. rename select (hb_priv_i bijb = hb_priv_i bijb') into Heq. rewrite -Heq.
+              move => ??? /=. rewrite lookup_union_r. 2: {
+                apply map_filter_lookup_None. right => ?? /=. admit. }
+              rewrite map_filter_lookup_true; [by apply Hprevb|].
+              move => ?? /=. right. move => /elem_of_hb_shared_i[??].
+              efeed pose proof hb_disj as HNone; [done|]. rewrite -Heq in HNone. naive_solver.
+           ++ iIntros (p1 p2 o ?) => /=.
+              destruct (decide (p1 ∈ dom (gset _) (ih' ∪ i2a_ih_shared iha))).
+              ** rewrite lookup_union_l'.
+                 2: { apply map_filter_lookup_None. right => ?? /=. rewrite elem_of_hb_shared_i. naive_solver. }
+                 admit. (* tricky *)
+              ** rewrite lookup_union_r. 2: { apply map_filter_lookup_None. naive_solver. }
+                 admit. (* tricky *)
+        -- rewrite big_sepL2_fmap_l. iApply big_sepL_sepL2_diag.
+           iDestruct "Hsh" as "#Hsh".
+           iApply big_sepL_intro. iIntros "!>" (???).
+           revert select (i2a_args_pure  _ _ _ _) => /(_ _ _ ltac:(done))[?[?[?[??]]]].
+           by iApply (val_in_through_bij with "[$]").
+      * iSatMono HP'. iIntros!. iFrame.
+        admit.
+      * by apply map_subseteq_difference_l.
+    + move => v av rs' cs' ?? P' HP'. eexists false => /=. simplify_eq. setoid_subst.
+      rename select (satisfiable (Pa ∗ _)) into HPa.
+      rename select (satisfiable (Pb ∗ _)) into HPb.
+      rename select (i2a_heap_agree hprev iha) into Hpa.
+      iSatStart HP'. iIntros!.
+      iDestruct select (i2a_mem_inv _ _ _) as (?) "(Hgp&Hsp&Hmauth)".
+      iDestruct (i2a_mem_lookup_big' mo with "[$] [$]") as %?.
+      iDestruct (i2a_mem_uninit_alt1 with "[$]") as (? Hvslen) "Hsp"; [lia|].
+      iDestruct select (i2a_heap_inv _) as (ih ?) "[Hsh [Hhag Hh]]".
+      iDestruct (i2a_heap_shared_lookup_big1 with "[$] [$]") as %?.
+      iDestruct (i2a_heap_shared_lookup_big1 (i2a_combine_bij _ _) with "[$] [$]") as %?.
+      iDestruct (i2a_heap_lookup_big1 with "[$] [$]") as %?.
+      iDestruct (i2a_heap_shared_agree_to_pure with "[$] [$]") as (??) "[? ?]".
+      iDestruct (i2a_val_rel_to_pure with "[$] [$]") as %?.
+      iSatStop HP'.
+
+      have [//|//|//|//|ih' [bijb' ?]]:= i2a_combine_extend iha bijb ih ho h. destruct_all?.
+
+      iSatStartBupd HPa. iIntros!.
+      iMod (i2a_mem_update_all1 mem with "[$] [$]") as "[Ha Hmo]"; [done..|].
+      iMod (i2a_heap_alloc_shared_big1 with "[$]") as "[Hih ?]"; [done..|]. iModIntro.
+      iSatStop HPa.
+      efeed pose proof i2a_mem_transfer as H'.
+      2: { iSatMono HPa. iFrame. iAccu. }
+      { iSatMono HP'. iFrame. iAccu. }
+      clear HPa HP'. move: H' => [HP' HPa].
+      efeed pose proof i2a_mem_transfer as H'.
+      2: { iSatMono HPa. iIntros!. iFrame. iAccu. }
+      { iSatMono HP'. iIntros!. iFrame. iAccu. }
+      clear HPa HP'. move: H' => [HP' HPa].
+      efeed pose proof i2a_mem_transfer as H'.
+      2: { iSatMono HPa. iIntros!. iFrame. iAccu. }
+      { iSatMono HP'. iIntros!. iFrame. iAccu. }
+      clear HPa HP'. move: H' => [HP' HPa].
+      split; [done|].
+      eexists (heap_merge (heap_restrict (heap_through_bij bijb' h)
+                                         (λ p, p ∈ ih' ∪ i2a_ih_shared iha))
+                  (heap_restrict hprev
+                                 (λ x, x ∉ ih' ∪ i2a_ih_shared iha ∨ x ∉ hb_shared_i bijb'))).
+      eexists (val_through_bij bijb' v).
+      split!.
+      * done.
+      * iSatMono HPa. iIntros!.
+        iDestruct select (i2a_mem_map (mem ∖ _)) as "$". iFrame.
+        rewrite -!(assoc bi_sep). iSplit; [done|].
+        iDestruct (i2a_mem_uninit_alt2 with "[$]") as "Huninit". rewrite Hvslen Z2Nat.id; [|lia].
+        iFrame "Huninit".
+        rewrite !bi.sep_exist_r. iExists _.
+        rewrite -!(assoc bi_sep).
+        iDestruct select (i2a_heap_auth _) as "$".
+        iAssert ([∗ map] p↦a ∈ i2a_ih_shared ((I2AShared <$> ih') ∪ iha), i2a_heap_shared p a)%I as "#$". {
+          admit.
+        }
+
+        iSplit!.
+        -- split.
+           ++ rewrite heap_merge_provs !heap_restrict_provs dom_union_L. admit.
+           ++ move => /= ?? /lookup_union_Some_raw. rewrite lookup_fmap.
+              move => [/fmap_Some[?[?//]]|[/fmap_None ??]]. rewrite lookup_union_r. 2: {
+                apply map_filter_lookup_None. right => ?? /=. admit. }
+              rewrite map_filter_lookup_true; [by apply Hpa|].
+              admit.
+        -- admit. (* TODO, not clear yet *)
+        -- iApply (i2a_val_rel_of_pure (ih' ∪ i2a_ih_shared iha)).
+           ++ by apply: i2a_val_rel_pure_through_bij.
+           ++ by iApply (big_sepM_union_2 with "[$]").
+      * iSatMono HPb. iIntros!. iFrame.
+        admit.
+      * by instantiate (1:= [_]).
+      * iSatMono HP'. iIntros!. iFrame.
+        admit.
+      * by apply map_subseteq_difference_l.
+  - move => vs hb' Pb' HPb' ? i rs' mem''.
     destruct e as [fn args h|v h]; simplify_eq/=.
-    + move => ret ????? Pa' HPa'.
+    + move => ret ????? Pa' HPa'. setoid_subst.
       (* split!. *)
       admit.
-    + move => av lr' cs' ??? Pa' HPa'. simplify_eq/=.
+    + move => av lr' cs' ??? Pa' HPa'. simplify_eq/=. setoid_subst.
       (* split!. *)
       admit.
 Admitted.
